proof/DDC/Language/SimpleRef/Eval.v
@@ -1,0 +1,165 @@
+
+Require Export DDC.Language.SimpleRef.SubstExpExp.
+Require Import DDC.Language.SimpleRef.Preservation.
+Require Import DDC.Language.SimpleRef.Ty.
+Require Export DDC.Language.SimpleRef.Step.
+Require Export DDC.Language.SimpleRef.Exp.
+
+
+(********************************************************************)
+(** Big Step Evaluation *)
+(*  This is also called 'Natural Semantics'.
+    It provides a relation between the expression to be reduced 
+    and its final value. 
+ *)
+Inductive EVAL : exp -> exp -> Prop :=
+ | EVDone
+   :  forall v2
+   ,  wnfX  v2
+   -> EVAL   v2 v2
+
+ | EVLamApp
+   :  forall x1 t11 x12 x2 v2 v3
+   ,  EVAL x1 (XLam t11 x12) -> EVAL x2 v2 -> EVAL (substX 0 v2 x12) v3
+   -> EVAL (XApp x1 x2) v3.
+
+Hint Constructors EVAL.
+
+
+(* A terminating big-step evaluation always produces a whnf.
+   The fact that the evaluation terminated is implied by the fact
+   that we have a finite proof of EVAL to pass to this lemma. 
+ *)
+Lemma eval_produces_whnfX
+ :  forall x1 v1
+ ,  EVAL   x1 v1
+ -> wnfX  v1.
+Proof.
+ intros. induction H; eauto.
+Qed.
+Hint Resolve eval_produces_whnfX.
+
+
+(********************************************************************)
+(** * Big to Small steps *)
+(* Convert a big-step evaluation into a list of individual
+   machine steps.
+ *)
+Lemma steps_of_eval
+ :  forall x1 t1 x2
+ ,  TYPE nil x1 t1
+ -> EVAL  x1 x2
+ -> STEPS x1 x2.
+Proof.
+ intros x1 t1 v2 HT HE. gen t1.
+
+ (* Induction over the form of (EVAL x1 x2) *)
+ induction HE.
+ Case "EVDone".
+  intros. apply EsNone.
+
+ Case "EVLamApp".
+  intros. inverts HT.
+
+  lets E1: IHHE1 H2. 
+  lets E2: IHHE2 H4.
+
+  lets T1: preservation_steps H2 E1. inverts keep T1.
+  lets T2: preservation_steps H4 E2.
+  lets T3: subst_exp_exp H1 T2.
+  lets E3: IHHE3 T3.
+
+  eapply EsAppend.
+    lets D: steps_context XcApp1. eapply D. eauto.
+   eapply EsAppend.
+    lets D: steps_context XcApp2 E2; eauto.
+   eapply EsAppend.
+    eapply EsStep.
+     eapply EsLamApp. eauto.
+   eauto.
+Qed.
+
+
+(********************************************************************)
+(** * Small to Big steps *)
+(** Convert a list of individual machine steps to a big-step
+    evaluation. The main part of this is the expansion lemma, which 
+    we use to build up the overall big-step evaluation one small-step
+    at a time. The other lemmas are used to feed it small-steps.
+ *)
+
+(* Given an existing big-step evalution, we can produce a new one
+   that does an extra step before returning the original value.
+ *)
+Lemma eval_expansion
+ :  forall te x1 t1 x2 v3
+ ,  TYPE te x1 t1
+ -> STEP x1 x2 -> EVAL x2 v3 
+ -> EVAL x1 v3.
+Proof.
+ intros. gen te t1 v3.
+
+ (* Induction over the form of (STEP x1 x2) *)
+ induction H0; intros.
+
+ Case "eval in context".
+  destruct H. 
+
+  SCase "top level".
+   eauto.
+ 
+  SCase "x1 steps".
+   inverts H1. inverts H2.
+    inverts H.
+    eapply EVLamApp; eauto.
+
+  SCase "x2 steps".
+   inverts H1. inverts H2.
+   inverts H1.
+   eapply EVLamApp; eauto.
+
+  SCase "application".
+   eapply EVLamApp.
+    eauto.
+    inverts H. 
+    apply EVDone. auto. auto.
+Qed.
+
+
+(* Convert a list of small steps to a big-step evaluation. *)
+Lemma eval_of_stepsl
+ :  forall x1 t1 v2
+ ,  TYPE nil x1 t1
+ -> STEPSL   x1 v2 -> value v2
+ -> EVAL     x1 v2.
+Proof.
+ intros.
+ induction H0.
+ 
+ Case "ESLNone".
+   apply EVDone. inverts H1. auto.
+
+ Case "ESLCons".
+  eapply eval_expansion. 
+   eauto. eauto. 
+   apply IHSTEPSL.
+   eapply preservation. eauto. auto. auto.
+Qed.
+
+
+(* Convert a multi-step evaluation to a big-step evaluation.
+   We use stepsl_of_steps to flatten out the append constructors
+   in the multi-step evaluation, leaving a list of individual
+   small-steps.
+ *)
+Lemma eval_of_steps
+ :  forall x1 t1 v2
+ ,  TYPE nil x1 t1
+ -> STEPS x1 v2 -> value v2
+ -> EVAL  x1 v2.
+Proof.
+ intros.
+ eapply eval_of_stepsl; eauto.
+ apply  stepsl_of_steps; auto.
+Qed.
+
