proof/DDC/Language/SimpleRef/Exp.v
@@ -1,0 +1,197 @@
+Require Export DDC.Base.
+
+(********************************************************************)
+(* Types *)
+Inductive ty  : Type :=
+ | TCon  : nat -> ty               (* data type constructor *)
+ | TFun  : ty  -> ty -> ty         (* function type constructor *)
+ | TRef  : ty  -> ty.              (* reference type constructor *)
+Hint Constructors ty.
+
+(* Baked in types. *)
+Definition tUnit  := TCon 0.
+
+(* Type Environment. *)
+Definition tyenv := list ty.
+
+(* Store typing. *)
+Definition stenv := list ty.
+
+
+(********************************************************************)
+(* Value Expressions *)
+Inductive exp : Type :=
+ (* Base calculus. *)
+ | XCon      : nat  -> exp         (* data constructor *)
+ | XVar      : nat  -> exp         (* deBruijn index *)
+ | XLam      : ty   -> exp -> exp  (* function abstraction *)
+ | XApp      : exp  -> exp -> exp  (* function application *)
+
+ (* Primitive operators.
+    We want to define these in fully applied form because so we don't
+    need to worry about partial application in the typing rules. We
+    can't use XApp directly becuase the primitives need to be
+    polymorphic but we only have a monomorphic base calculus. *)
+ | XNewRef   : exp -> exp          (* allocate a new reference *)
+ | XReadRef  : exp -> exp          (* read a references *)
+ | XWriteRef : exp -> exp -> exp   (* write to a reference *)
+
+ (* Expressions created during reduction, 
+    and not usually part of the initial program. *)
+ | XLoc      : nat  -> exp.         (* store location *)
+Hint Constructors exp.
+
+
+(* Baked in expressions *)
+Definition xUnit := XCon 0.
+
+
+(* Heap *)
+Definition heap := list exp.
+
+
+(* Weak normal forms.
+   Expressions in weak normal form cannot be reduced further by
+   call-by-value evaluation. *)
+Inductive wnfX : exp -> Prop :=
+ | Wnf_XVar 
+   : forall i
+   , wnfX (XVar i)
+
+ | Wnf_XLam
+   : forall t1 x2
+   , wnfX (XLam t1 x2)
+
+ | Wnf_XLoc
+   : forall l
+   , wnfX (XLoc l).
+Hint Constructors wnfX.
+
+
+(* Well formed expressions are closed under the given environment. *)
+Fixpoint wfX (te: tyenv) (xx: exp) : Prop :=
+ match xx with  
+ | XCon _          => True
+ | XVar i          => exists t, get i te = Some t
+ | XLam t x        => wfX (te :> t) x
+ | XApp x1 x2      => wfX te x1 /\ wfX te x2
+ | XNewRef x       => wfX te x
+ | XReadRef x      => wfX te x
+ | XWriteRef x1 x2 => wfX te x1 /\ wfX te x2
+ | XLoc _          => True
+ end.
+
+
+(* Closed expressions are well formed under an empty environment. *)
+Definition closedX (xx: exp) : Prop
+ := wfX nil xx.
+Hint Unfold closedX.
+
+
+(* Values are closed expressions that cannot be reduced further. *)
+Inductive value : exp -> Prop :=
+ | Value 
+   :  forall xx
+   ,  wnfX xx -> closedX xx
+   -> value xx.
+Hint Constructors value.
+
+
+(********************************************************************)
+(* Lifting of references into the environment.
+   When we push new elements on the environment stack, we need
+   to lift referenes to existing elements across the new ones. 
+
+   For example given: 
+             t1, t0 |- 0 1 (\. 0 1 2) :: t3
+
+   Pushing two more elements gives:
+     t1, t0, ta, tb |- 2 3 (\. 0 3 4) :: t3
+ *)
+Fixpoint 
+ liftX  (d:  nat) (* current binding depth in expression *)
+        (xx: exp) (* expression containing referenes to lift *)
+        : exp
+ := match xx with 
+    |  XCon i
+    => XCon i
+
+    |  XVar ix    
+    => if le_gt_dec d ix
+        (* Index is referencing the env, so lift it across the new elem *)
+        then XVar (S ix)
+
+        (* Index is locally bound in the expression itself, and 
+           not the environment, so we don't need to change it. *)
+        else xx
+
+    (* Increase the current depth as we move across a lambda, 
+       if we find locally bound indices that reference this lambda
+       then we don't need to lift them. *)
+    |  XLam t1 x1
+    => XLam t1 (liftX (S d) x1)
+
+    |  XApp x1 x2
+    => XApp   (liftX d x1) (liftX d x2)
+
+    |  XNewRef x1 
+    => XNewRef (liftX d x1)
+
+    |  XReadRef x1
+    => XReadRef (liftX d x1)
+ 
+    |  XWriteRef x1 x2
+    => XWriteRef (liftX d x1) (liftX d x2)
+
+    |  XLoc  l  
+    => XLoc  l
+    end.
+
+
+(*******************************************************************)
+(* Substitute for the outermost binder in an expression. *)
+Fixpoint
+ substX (d:  nat) (* current binding depth in expression *)
+        (u:  exp) (* new expression to substitute *)
+        (xx: exp) (* expression to substitute into *)
+        : exp 
+ := match xx with
+    |  XCon i
+    => XCon i
+
+    | XVar ix 
+    => match nat_compare ix d with
+       (* Index matches the one we are substituting for. *)
+       | Eq  => u
+       
+       (* Index was free in the original expression.
+          As we've removed the outermost binder, also decrease this
+          index by one. *)
+       | Gt  => XVar (ix - 1)
+
+       (* Index was bound in the original expression. *)
+       | Lt  => XVar ix
+       end
+
+    (* Increase the depth as we move across a lambda.
+       Any free references in the exp being substitued also need
+       to be lifted across the lambda as we enter it. *)
+    |  XLam t1 x2
+    => XLam t1 (substX (S d) (liftX 0 u) x2)
+
+    |  XApp x1 x2 
+    => XApp (substX d u x1) (substX d u x2)
+
+    |  XNewRef x1
+    => XNewRef (substX d u x1)
+
+    |  XReadRef x1
+    => XReadRef (substX d u x1)
+
+    |  XWriteRef x1 x2
+    => XWriteRef (substX d u x1) (substX d u x2)
+    
+    |  XLoc l
+    => XLoc l
+ end. 
+
