proof/DDC/Language/SimpleRef/Preservation.v
@@ -1,0 +1,61 @@
+
+Require Import DDC.Language.SimpleRef.Step.
+Require Import DDC.Language.SimpleRef.SubstExpExp.
+Require Import DDC.Language.SimpleRef.Ty.
+
+
+(* If a closed, well typed expression takes an evaluation step 
+   then the result has the same type as before. *)
+Theorem preservation
+ :  forall x x' t
+ ,  TYPE nil x  t
+ -> STEP x x'
+ -> TYPE nil x' t.
+Proof.
+ intros. gen t.
+ induction H0; intros.
+
+ Case "EsContext".
+  destruct H.
+  eauto.
+  inverts H1. eauto.
+  inverts H1. eauto.
+
+ Case "EsLamApp".
+  inverts H0.
+  inverts H4.
+  eapply subst_exp_exp; eauto.
+Qed.
+
+
+(* If a closed, well typed expression takes several evaluation steps
+   then the result has the same type as before. *)
+Lemma preservation_steps
+ :  forall x1 t1 x2
+ ,  TYPE nil x1 t1
+ -> STEPS    x1 x2
+ -> TYPE nil x2 t1.
+Proof.
+ intros. 
+ induction H0; eauto.
+  eapply preservation; eauto.
+Qed.
+
+
+(* If a closed, well typed expression takes several evaluation steps
+   then the result has the same type as before. 
+   Usses the left linearised version of steps judement. *)
+Lemma preservation_stepsl
+ :  forall x1 t1 x2
+ ,  TYPE nil x1 t1
+ -> STEPSL   x1 x2
+ -> TYPE nil x2 t1.
+Proof.
+ intros. 
+ induction H0.
+  auto.
+  apply IHSTEPSL.
+  eapply preservation. 
+   eauto. auto.
+Qed.
+
