proof/DDC/Language/SimpleRef/Progress.v
@@ -1,0 +1,122 @@
+
+Require Import DDC.Language.SimpleRef.Step.
+Require Import DDC.Language.SimpleRef.Ty.
+Require Import DDC.Language.SimpleRef.Exp.
+
+Lemma value_ref
+ :  forall x te se t
+ ,  value x
+ -> TYPE te se x (TRef t)
+ -> (exists l, x = XLoc l).
+Proof.
+ intros.
+ destruct x; try (inverts H0); try (inverts H; inverts H0).
+ inverts H1. inverts H.
+ inverts H1. eauto.
+Qed.
+Hint Resolve value_ref.
+
+
+(* A closed, well typed expression is either a value or can 
+   take a step in the evaluation. *)
+Theorem progress
+ :  forall se h x t
+ ,  TYPEH se h
+ -> TYPE  nil se x t
+ -> value x \/ (exists h' x', STEP h x h' x').
+Proof.
+ intros se h x t HTH HT.
+ remember (@nil ty) as tyenv.
+ induction HT.
+
+ Case "XVar".
+  subst. inverts H.
+
+ Case "XLoc".
+  left. eauto.
+
+ Case "XLam".
+  left. subst. eauto.
+
+ Case "XApp".
+  right. 
+  specializes IHHT1 Heqtyenv. auto.
+  specializes IHHT2 Heqtyenv. auto.
+  destruct IHHT1.
+
+  SCase "value x1".
+   destruct IHHT2.
+   SSCase "value x2".
+    inverts H. inverts H1.
+     inverts H2. false.
+     SSSCase "EsLamApp".
+      exists h.
+      exists (substX 0 x2 x0).
+      apply EsLamApp. auto.
+     SSSCase "XLoc".
+      inverts HT1.
+
+   SSCase "x2 steps".
+    destruct H0 as [h'].
+    destruct H0 as [x2'].
+    exists h'. exists (XApp x1 x2'). 
+    inverts H. auto.
+
+   SSCase "x1 steps".
+    destruct H as [h'].
+    destruct H as [x1'].
+    exists h'. exists (XApp x1' x2).
+    lets D: EsContext XcApp1. eauto.
+
+ Case "XNewRef".
+  right.
+  destruct IHHT; eauto.
+  SCase "x1 steps".
+   destruct H as [h'].
+   destruct H as [xData'].
+   exists h'. exists (XNewRef xData'). auto.
+
+ Case "XReadRef".
+  right.
+  destruct IHHT; eauto.
+  SCase "xRef value".
+   subst. 
+   assert (exists l, xRef = XLoc l). eauto.
+    destruct H0 as [l]. subst.
+
+   inverts HT.
+   assert (exists xData, get l h = Some xData).
+    admit. destruct H0 as [xData]. (* ok, list lemma *)
+
+   exists h.
+   exists xData. auto.
+
+  SCase "xRef steps".
+   destruct H as [h'].
+   destruct H as [x'].
+   exists h' (XReadRef x').
+   lets D: EsContext XcReadRef. eauto.
+
+ Case "XWriteRef".
+  right.
+  specializes IHHT1 Heqtyenv. auto.
+  specializes IHHT2 Heqtyenv. auto.
+
+  destruct IHHT1.
+  SCase "value xRef".
+   destruct IHHT2.
+    SSCase "value xData".
+     assert (exists l, xRef = XLoc l). eauto.
+     destruct H1 as [l]. subst.
+     exists (update l xData h). exists xUnit.
+     auto.
+    SSCase "x2 steps".
+     destruct H0 as [h']. exists h'.
+     destruct H0 as [xData'].
+      exists (XWriteRef xRef xData'). auto.
+      inverts H. auto. 
+   SCase "xRef Steps".
+    destruct H as [h']. 
+    destruct H as [xRef']. 
+     lets D: EsContext XcWriteRef1. eauto. 
+Qed.
