proof/DDC/Language/SimpleRef/Step.v
@@ -1,0 +1,183 @@
+
+Require Export DDC.Language.SimpleRef.SubstExpExp.
+Require Export DDC.Language.SimpleRef.Exp.
+
+
+(*******************************************************************)
+(* Evaluation contexts for expressions.
+   An evaluation context is an expression with a hole in any place
+   that can take a step via our evaluatio rules. We represent
+   the hole by the function that fills it. 
+ *)
+Inductive exp_ctx : (exp -> exp) -> Prop :=
+ | XcTop
+   :  exp_ctx (fun x => x)
+
+ | XcApp1
+   :  forall x2
+   ,  exp_ctx (fun xx => XApp xx x2)
+
+ | XcApp2 
+   :  forall v1
+   ,  wnfX v1 
+   -> exp_ctx (fun xx => XApp v1 xx)
+
+ | XcNewRef
+   :  exp_ctx (fun xx => XNewRef xx)
+
+ | XcReadRef
+   :  exp_ctx (fun xx => XReadRef xx)
+
+ | XcWriteRef1
+   :  forall x2
+   ,  exp_ctx (fun xx => XWriteRef xx x2)
+
+ | XcWriteRef2
+   :  forall v1
+   ,  wnfX v1
+   -> exp_ctx (fun xx => XWriteRef v1 xx).
+
+Hint Constructors exp_ctx.
+
+
+
+(* Small Step evaluation *)
+Inductive STEP  : heap -> exp -> heap -> exp -> Prop :=
+
+ (* Evaluation in a context. *)
+ | EsContext 
+   :  forall C h x h' x'
+   ,  exp_ctx C
+   -> STEP h x     h' x'
+   -> STEP h (C x) h' (C x')
+
+ (* Function application. *)
+ | EsLamApp 
+   :  forall h t11 x12 v2
+   ,  value v2
+   -> STEP h (XApp (XLam t11 x12) v2)
+           h (substX 0 v2 x12)
+
+ (* References *)
+ | EsNewRef
+   :  forall h v1
+   ,  value v1
+   -> STEP h         (XNewRef v1)
+           (h :> v1) (XLoc (length h))
+
+ | EsReadRef
+   :  forall l h v
+   ,  get l h = Some v
+   -> STEP h  (XReadRef (XLoc l))
+           h  v
+
+ | EsWriteRef
+   :  forall l h v2
+   ,  STEP h  (XWriteRef (XLoc l) v2)
+           (update l v2 h) xUnit.
+
+Hint Constructors STEP.
+
+
+(********************************************************************)
+(* Multi-step evaluation
+   A sequence of small step transitions.
+   As opposed to STEPSL, this version has an append constructor
+   EsAppend that makes it easy to join two evaluations together.
+   We use this when converting big-step evaluations to small-step.
+ *)
+Inductive STEPS : heap -> exp -> heap -> exp -> Prop :=
+
+ (* After no steps, we get the same exp.
+    We need this constructor to match the EVDone constructor
+    in the big-step evaluation, so we can convert between big-step
+    and multi-step evaluations. *)
+ | EsNone
+   :  forall h x
+   ,  STEPS h x  h x
+
+ (* Take a single step. *)
+ | EsStep
+   :  forall h1 x1 h2 x2
+   ,  STEP  h1 x1 h2 x2
+   -> STEPS h1 x1 h2 x2
+
+ (* Combine two evaluations into a third. *)
+ | EsAppend
+   :  forall h1 x1 h2 x2 h3 x3
+   ,  STEPS h1 x1 h2 x2 -> STEPS h2 x2 h3 x3
+   -> STEPS h1 x1 h3 x3.
+
+Hint Constructors STEPS.
+
+
+(* Multi-step evaluation in a context.
+   If an expression can be evaluated at top level, then it can 
+   be evaluated to the same result in any evaluation context. *)
+Lemma steps_context
+ :  forall C h x h' x'
+ ,  exp_ctx C
+ -> STEPS h x     h' x'
+ -> STEPS h (C x) h' (C x').
+Proof.
+ intros.
+ induction H0.
+  auto.
+  auto.
+  eapply EsAppend. eauto. eauto.
+Qed.
+
+
+(********************************************************************)
+(* Left linearised multi-step evaluation
+   As opposed to STEPS, this version provides a single step at a time
+   and does not have an append constructor. This is convenient
+   when converting a small-step evaluations to big-step, via the
+   eval_expansion lemma.
+ *)
+Inductive STEPSL : heap -> exp -> heap -> exp -> Prop :=
+
+ | EslNone 
+   : forall h x
+   , STEPSL h x h x
+
+ | EslCons
+   :  forall h1 x1 h2 x2 h3 x3
+   ,  STEP   h1 x1 h2 x2 -> STEPSL h2 x2 h3 x3 
+   -> STEPSL h1 x1 h3 x3.
+
+Hint Constructors STEPSL.
+
+
+(* Transitivity of left linearised multi-step evaluation.
+   We use this when "flattening" a big step evaluation to the
+   small step one.
+ *)
+Lemma stepsl_trans
+ :  forall h1 x1 h2 x2 h3 x3
+ ,  STEPSL h1 x1 h2 x2 -> STEPSL h2 x2 h3 x3
+ -> STEPSL h1 x1 h3 x3.
+Proof.
+ intros.
+ induction H.
+  eauto.
+  eapply EslCons. eauto. eauto.
+Qed.
+
+
+(* Linearise a regular multi-step evaluation.
+   This flattens out all the append constructors, leaving us with
+   a list of individual transitions. 
+ *)
+Lemma stepsl_of_steps
+ :  forall h1 x1 h2 x2
+ ,  STEPS  h1 x1 h2 x2
+ -> STEPSL h1 x1 h2 x2.
+Proof. 
+ intros.
+ induction H.
+  auto.
+  eauto.
+  eapply stepsl_trans; eauto.
+Qed.
+
