proof/DDC/Language/SimpleRef/SubstExpExp.v
@@ -1,0 +1,56 @@
+
+Require Import DDC.Language.SimpleRef.Ty.
+Require Export DDC.Language.SimpleRef.Exp.
+
+(* Substitution of expressions in expressions preserves typing.
+
+   Inductively, we must reason about performing substitutions at any
+   depth, hence we must prove a property about (subst' d x2 x1) instead
+   of the weaker (subst x2 x1) which assumes the substitution is taking
+   place at top level. *)
+Lemma subst_exp_exp_ix
+ :  forall ix te se x1 x2 t1 t2
+ ,  get  ix te = Some t2
+ -> TYPE te se             x1 t1
+ -> TYPE (delete ix te) se x2 t2
+ -> TYPE (delete ix te) se (substX ix x2 x1) t1.
+Proof.
+ intros. gen ix te se x2 t1.
+ induction x1; intros; simpl; inverts H0; eauto.
+
+ Case "XVar".
+  fbreak_nat_compare.
+  SCase "i = ix".
+   rewrite H in H5. inverts H5. auto.
+
+  SCase "n < ix".
+   apply TyVar.
+   rewrite <- H5.
+    apply get_delete_above. auto.
+
+  SCase "n > ix".
+   apply TyVar.
+   destruct n.
+    false. omega.
+    simpl. nnat. rewrite <- H5.
+     apply get_delete_below. omega.
+
+ Case "XLam".
+  apply TyLam.
+  rewrite delete_rewind.
+  apply IHx1; auto.
+   simpl. apply type_tyenv_weaken. auto.
+Qed.
+
+
+Theorem subst_exp_exp
+ :  forall te se x1 x2 t1 t2
+ ,  TYPE (te :> t2) se x1 t1
+ -> TYPE te se         x2 t2 
+ -> TYPE te se (substX 0 x2 x1) t1.
+Proof. 
+ intros te se x1 x2 t1 t2 Ht1 Ht2.
+ lets H: subst_exp_exp_ix 0 (te :> t2).
+  simpl in H. eauto.
+Qed.
+
