proof/DDC/Language/SimpleRef/Ty.v
@@ -1,0 +1,100 @@
+
+Require Export DDC.Language.SimpleRef.Exp.
+
+(* Typing judgement assigns a type to an expression. *)
+Inductive TYPE : tyenv -> stenv -> exp -> ty -> Prop :=
+ | TyVar 
+   :  forall te se i t
+   ,  get i te = Some t
+   -> TYPE te se (XVar i) t
+
+ | TyLoc
+   :  forall te se i t
+   ,  get i se = Some t
+   -> TYPE te se (XLoc i) (TRef t)
+
+ | TyLam
+   :  forall te se x t1 t2
+   ,  TYPE (te :> t1) se x t2
+   -> TYPE te se (XLam t1 x) (TFun t1 t2)
+
+ | TyApp
+   :  forall te se x1 x2 t1 t2
+   ,  TYPE te se x1 (TFun t1 t2)
+   -> TYPE te se x2 t1
+   -> TYPE te se (XApp x1 x2) t2
+
+ (* As these primitives are polymorphic, 
+    but we're using a monomorphic ambient calculus
+    we must give them their own rules. *)
+ | TyNewRef
+   :  forall te se xData tData
+   ,  TYPE te se xData tData
+   -> TYPE te se (XNewRef xData)  (TRef tData)
+
+ | TyReadRef
+   :  forall te se xRef tData
+   ,  TYPE te se xRef (TRef tData)
+   -> TYPE te se (XReadRef xRef)  tData
+
+ | TyWriteRef
+   :  forall te se xRef xData tData 
+   ,  TYPE te se xRef  (TRef tData)
+   -> TYPE te se xData tData
+   -> TYPE te se (XWriteRef xRef xData) tUnit.
+
+Hint Constructors TYPE.
+
+
+(********************************************************************)
+Definition TYPEH (se : tyenv) (h: heap)
+   := Forall2 (TYPE nil nil) h se.
+
+
+(********************************************************************)
+(* A well typed expression is well formed. *)
+Theorem type_wfX
+ :  forall te se x t
+ ,  TYPE te se x t
+ -> wfX  te x.
+Proof.
+ intros. 
+ induction H; simpl; eauto.
+Qed.
+Hint Resolve type_wfX.
+
+
+(* Weakening the type environment of a typing judgement.
+   We can insert a new type into the type environment, provided we
+   lift existing references to types higher in the stack across
+   the new one. *)
+Lemma type_tyenv_insert
+ :  forall te se ix x t1 t2
+ ,  TYPE te se x t1
+ -> TYPE (insert ix t2 te) se (liftX ix x) t1.
+Proof.
+ intros. gen ix te se t1.
+ induction x; intros; simpl; inverts H; eauto.
+
+ Case "XVar".
+  lift_cases; intros; auto.
+
+ Case "XLam".
+  apply TyLam.
+  rewrite insert_rewind. 
+   apply IHx. auto.
+Qed.
+
+
+Lemma type_tyenv_weaken
+ :  forall te se x t1 t2
+ ,  TYPE  te se         x          t1
+ -> TYPE (te :> t2) se (liftX 0 x) t1.
+Proof.
+ intros.
+ assert (te :> t2 = insert 0 t2 te).
+  simpl. destruct te; auto.
+  rewrite H0. apply type_tyenv_insert. auto.
+Qed.
+
+
